Set up some indirect inode basics

src/Dafny/examples/fs/indirect_fs.dfy
@@ -10,32 +10,6 @@ module IndFs
   import opened Marshal
   import C = Collections
 
-  datatype IndBlock = IndBlock(bn: Blkno, blknos: seq<Blkno>)
-  {
-    predicate Valid()
-    {
-      && blkno_ok(bn)
-      && |blknos| == 512
-      && (forall k: int | 0 <= k < 512 :: blkno_ok(blknos[k]))
-    }
-
-    // helps state uniqueness (not just over this IndBlock but all blocks
-    // involved in an inode)
-    function all_blknos(): seq<Blkno>
-    {
-      [bn] + blknos
-    }
-
-    predicate in_fs(fs: Filesys)
-      reads fs.Repr()
-      requires fs.Valid()
-      requires Valid()
-    {
-      var b := zero_lookup(fs.data_block, this.bn);
-      && block_has_blknos(b, this.blknos)
-    }
-  }
-
   predicate block_has_blknos(b: Block, blknos: seq<Blkno>)
   {
     && is_block(b)
@@ -83,27 +57,168 @@ module IndFs
     return;
   }
 
+  datatype Idx = direct(k: nat) | indirect(k: nat, m: nat)
+  {
+    predicate Valid()
+    {
+      match this {
+        case direct(k) => k < 10
+        case indirect(k, m) => k < 5 && m < 512
+      }
+    }
+
+    function flat(): nat
+      requires Valid()
+    {
+      match this {
+        case direct(k) => k
+        case indirect(k, m) => 10 + k * 512 + m
+      }
+    }
+
+    static function from_flat(n: nat): (i:Idx)
+      requires n < 10 + 5*512
+      ensures i.Valid()
+    {
+      if n < 10 then
+        direct(n)
+      else (
+        var x := n-10;
+        indirect(x/512, x % 512)
+      )
+    }
+
+    lemma to_from_flat()
+      requires Valid()
+      ensures from_flat(this.flat()) == this
+    {}
+
+    static lemma from_to_flat(n: nat)
+      requires n < 10 + 5*512
+      ensures from_flat(n).flat() == n
+    {}
+  }
+
+  datatype IndBlock = IndBlock(bn: Blkno, blknos: seq<Blkno>)
+  {
+    static const zero: IndBlock := IndBlock(0, C.repeat(0 as Blkno, 512))
+
+    predicate Valid()
+    {
+      && blkno_ok(bn)
+      && |blknos| == 512
+      && (forall k: int | 0 <= k < 512 :: blkno_ok(blknos[k]))
+    }
+
+    static lemma zero_ok()
+      ensures zero.Valid()
+    {}
+
+    static lemma zero_in_fs(fs: Filesys)
+      requires fs.Valid()
+      ensures zero.in_fs(fs)
+    {
+      zero_block_blknos();
+    }
+
+    predicate in_fs(fs: Filesys)
+      reads fs.Repr()
+      requires fs.Valid()
+      requires Valid()
+    {
+      var b := zero_lookup(fs.data_block, this.bn);
+      && block_has_blknos(b, this.blknos)
+    }
+  }
 
   datatype IndInodeData = IndInodeData(sz: nat, blks: seq<Block>)
   {
+    static const zero: IndInodeData := IndInodeData(0, C.repeat(block0, 10 + 5*512))
+
+    predicate Valid()
+    {
+      && sz <= Inode.MAX_SZ
+      && |blks| == 10 + 5 * 512
+    }
+
+    static lemma zero_valid()
+      ensures zero.Valid()
+    {}
   }
 
   class IndFilesys
   {
-    ghost var ind_blocks: map<Blkno, IndBlock>
+    ghost var ino_meta: map<Ino, seq<IndBlock>>
+    ghost var ino_data: map<Ino, IndInodeData>
     const fs: Filesys
 
-    predicate Valid()
-      reads fs.Repr()
+    function Repr(): set<object>
     {
-      && fs.Valid()
+      {this} + fs.Repr()
     }
 
-    constructor(fs: Filesys)
+    static predicate meta_valid?(meta: seq<IndBlock>)
+    {
+      && |meta| == 5
+      && (forall k: nat | k < 5 :: meta[k].Valid())
+    }
+
+    predicate ValidMeta()
+      reads this
+    {
+      && ino_dom(ino_meta)
+      && (forall ino | ino_ok(ino) :: meta_valid?(ino_meta[ino]))
+    }
+
+    predicate ValidData()
+      reads this
+    {
+      && ino_dom(ino_data)
+      && (forall ino | ino_ok(ino) :: ino_data[ino].Valid())
+    }
+
+    static predicate ino_ind_match?(d: InodeData, meta: seq<IndBlock>, id: IndInodeData, data_block: map<Blkno, Block>)
+      requires blkno_dom(data_block)
+      requires meta_valid?(meta)
+      requires id.Valid()
+    {
+      && d.Valid()
+      && id.sz == d.sz
+      && forall idx: Idx | idx.Valid() ::
+      (match idx {
+        case direct(k) => d.blks[k] == id.blks[idx.flat()]
+        case indirect(k, m) =>
+          zero_lookup(data_block, meta[k].blknos[m]) == id.blks[idx.flat()]
+      })
+    }
+
+    predicate {:opaque} Valid_ino_data()
+      reads this.Repr()
       requires fs.Valid()
+      requires ino_dom(ino_meta)
+      requires ino_dom(ino_data)
+      requires ValidMeta()
+      requires ValidData()
+    {
+      forall ino | ino_ok(ino) ::
+        ino_ind_match?(fs.inode_blks[ino], ino_meta[ino], ino_data[ino], fs.data_block)
+    }
+
+    predicate Valid()
+      reads this.Repr()
+    {
+      && fs.Valid()
+      && ValidMeta()
+      && ValidData()
+    }
+
+    constructor(d: Disk)
       ensures Valid()
     {
-      this.fs := fs;
+      this.fs := new Filesys.Init(d);
+      this.ino_meta := map ino: Ino | ino_ok(ino) :: C.repeat(IndBlock.zero, 5);
+      this.ino_data := map ino: Ino | ino_ok(ino) :: IndInodeData.zero;
+      IndInodeData.zero_valid();
     }
   }
 
